lean/FlowAnalysis/PromotionModel/Basic.lean
@@ -1,0 +1,211 @@
+module
+public import FlowAnalysis.PromotionChain.Basic
+public import FlowAnalysis.PromotionChain.JoinImpl
+public import FlowAnalysis.ValueVersion.Basic
+public import FlowAnalysis.PromotionModel.JoinTestedImpl
+public import FlowAnalysis.Types
+
+namespace FlowAnalysis
+
+open PromotionChain
+
+variable {τ : Type} [Γ : DartTypeRepr τ]
+
+local notation "PromotionChain" => PromotionChain (τ := τ)
+
+/-- The state of a promotable value at a particular point in a function's execution. -/
+@[ext]
+public structure PromotionModel where
+  promotedTypes : PromotionChain
+  tested : Finset τ
+  assigned : Bool
+  unassigned : Bool
+  version? : Option ValueVersion
+
+local notation "PromotionModel" => PromotionModel (τ := τ)
+
+namespace «PromotionModel»
+
+@[expose]
+public def currentType (pm : PromotionModel) (baseType : τ) :=
+  match pm.promotedTypes.val.getLast? with
+  | none => baseType
+  | some T => if T ≤ baseType then T else baseType
+
+@[expose]
+public def join (pm₁ pm₂ : PromotionModel) :
+    PromotionModel :=
+  ⟨pm₁.promotedTypes.join pm₂.promotedTypes,
+    pm₁.tested ∪ pm₂.tested,
+    pm₁.assigned ∧ pm₂.assigned,
+    pm₁.unassigned ∧ pm₂.unassigned,
+    ValueVersion.join pm₁.version? pm₂.version?⟩
+
+/-- The join operation is idempotent (`join pm pm = pm`). -/
+@[simp]
+public theorem join_self (pm : PromotionModel) : pm.join pm = pm := by
+  rcases pm; simp [join]
+
+public instance join.instIdempotentOp :
+    Std.IdempotentOp (join (τ := τ)) where
+  idempotent := join_self
+
+/-- The join operation is commutative (`join pm₁ pm₂ = join pm₂ pm₁`). -/
+public theorem join_comm (pm₁ pm₂ : PromotionModel) : pm₁.join pm₂ = pm₂.join pm₁ := by
+  simp [join, PromotionChain.join_comm, Finset.union_comm, Bool.and_comm, ValueVersion.join_comm]
+
+public instance join.instCommutative : Std.Commutative (join (τ := τ)) where
+  comm := join_comm
+
+/-- The join operation is associative (`join (join pm₁ pm₂) pm₃ = join pm₁ (join pm₂ pm₃)`). -/
+public theorem join_assoc (pm₁ pm₂ pm₃ : PromotionModel) :
+    (pm₁.join pm₂).join pm₃ = pm₁.join (pm₂.join pm₃) := by
+  simp [join, PromotionChain.join_assoc, Finset.union_assoc, Bool.and_assoc, ValueVersion.join_assoc]
+
+public instance join.instAssociative : Std.Associative (join (τ := τ)) where
+  assoc := join_assoc
+
+end «PromotionModel»
+
+open «PromotionModel»
+
+public structure PromotionModelImpl where
+  promotedTypes : List τ
+  tested : List τ
+  assigned : Bool
+  unassigned : Bool
+  version? : Option ValueVersion
+
+local notation "PromotionModelImpl" => PromotionModelImpl (τ := τ)
+
+@[expose]
+public def PromotionModelImpl.join (pmI₁ pmI₂ : PromotionModelImpl) : PromotionModelImpl :=
+  ⟨(joinPromotedTypesImpl pmI₁.promotedTypes pmI₂.promotedTypes : Id _).run,
+    joinTestedImpl pmI₁.tested pmI₂.tested,
+    pmI₁.assigned ∧ pmI₂.assigned,
+    pmI₁.unassigned ∧ pmI₂.unassigned,
+    ValueVersion.join pmI₁.version? pmI₂.version?
+  ⟩
+
+@[expose]
+public def PromotionModelImpl.promotedType? (pmI : PromotionModelImpl) : Option τ :=
+  pmI.promotedTypes.getLast?
+
+@[expose]
+public def PromotionModelImpl.currentType (pmI : PromotionModelImpl) (baseType : τ) :
+    τ :=
+  match pmI.promotedType? with
+  | none => baseType
+  | some T => if T ≤ baseType then T else baseType
+
+public structure PromotionModelImpl.refines (pmI : PromotionModelImpl) (pm : PromotionModel) :
+    Prop where
+  promotedTypes : pmI.promotedTypes = pm.promotedTypes.val
+  tested : ∀ T, T ∈ pmI.tested ↔ T ∈ pm.tested
+  assigned : pmI.assigned = pm.assigned
+  unassigned : pmI.unassigned = pm.unassigned
+  version? : pmI.version? = pm.version?
+
+@[simp]
+public theorem PromotionModelImpl.refines.promotedTypes' {pmI : PromotionModelImpl}
+    {pm : PromotionModel} (h : PromotionModelImpl.refines pmI pm) :
+    (pmI.promotedTypes = pm.promotedTypes.val) ↔ True := by
+  simp [h.promotedTypes]
+
+@[simp]
+public theorem PromotionModelImpl.refines.tested' {pmI : PromotionModelImpl} {pm : PromotionModel}
+    (h : PromotionModelImpl.refines pmI pm) : (∀ T, T ∈ pmI.tested ↔ T ∈ pm.tested) ↔ True := by
+  simp [h.tested]
+
+@[simp]
+public theorem PromotionModelImpl.refines.assigned' {pmI : PromotionModelImpl} {pm : PromotionModel}
+    (h : PromotionModelImpl.refines pmI pm) : (pmI.assigned = pm.assigned) ↔ True := by
+  simp [h.assigned]
+
+@[simp]
+public theorem PromotionModelImpl.refines.unassigned' {pmI : PromotionModelImpl} {pm : PromotionModel}
+    (h : PromotionModelImpl.refines pmI pm) : (pmI.unassigned = pm.unassigned) ↔ True := by
+  simp [h.unassigned]
+
+@[simp]
+public theorem PromotionModelImpl.refines.version?' {pmI : PromotionModelImpl} {pm : PromotionModel}
+    (h : PromotionModelImpl.refines pmI pm) : (pmI.version? = pm.version?) ↔ True := by
+  simp [h.version?]
+
+/--
+The promotion model that the algorithm creates for a freshly declared variable refines the
+promotion model that the specification creates for it.
+-/
+@[simp]
+public theorem PromotionModelImpl.refines.declared :
+    (⟨[], [], true, false, some ⟨⟩⟩ : PromotionModelImpl).refines
+      ⟨∅, ∅, true, false, some ⟨⟩⟩ := by
+  constructor <;> simp
+
+public theorem PromotionModelImpl.refines.unique {pmI : PromotionModelImpl}
+    {pm₁ pm₂ : PromotionModel} :
+    pmI.refines pm₁ → pmI.refines pm₂ → pm₁ = pm₂ := by
+  intro h₁ h₂
+  ext1
+  case promotedTypes => ext1; rw [←h₁.promotedTypes, ←h₂.promotedTypes]
+  case tested => ext; rw [←h₁.tested, ←h₂.tested]
+  case assigned => rw [←h₁.assigned, ←h₂.assigned]
+  case unassigned => rw [←h₁.unassigned, ←h₂.unassigned]
+  case version? => rw [←h₁.version?, ←h₂.version?]
+
+public theorem PromotionModelImpl.refines.currentTypes {pmI : PromotionModelImpl} {pm : PromotionModel}
+    {baseType : τ} : pmI.refines pm → pmI.currentType baseType = pm.currentType baseType := by
+  intro hrefines
+  simp [PromotionModelImpl.currentType, PromotionModelImpl.promotedType?, PromotionModel.currentType]
+  rw [hrefines.promotedTypes]
+
+/--
+Refinement implies that `pmI` and `pm` agree about whether a promotion to `T` is possible: appending
+`T` to `pmI`'s list of promoted types produces a valid promotion chain iff `pm`'s promotion chain
+strictly bounds `T`.
+-/
+public theorem PromotionModelImpl.refines.strictly_bounds_iff {pmI : PromotionModelImpl}
+    {pm : PromotionModel} {T : τ} (hrefines : pmI.refines pm) :
+    isPromotionChain (pmI.promotedTypes ++ [T]) ↔ pm.promotedTypes.strictly_bounds T := by
+  rw [PromotionChain.strictly_bounds, hrefines.promotedTypes]
+
+/--
+The algorithm promotes a variable to `T` by appending `T` to its list of promoted types, but only
+when the resulting list is a valid promotion chain. This theorem shows that doing so refines
+`PromotionChain.tryPromote`, which appends `T` under precisely the same circumstances.
+-/
+public theorem PromotionModelImpl.refines.promote {pmI : PromotionModelImpl} {pm : PromotionModel}
+    {T : τ} (hrefines : pmI.refines pm) (hchain : isPromotionChain (pmI.promotedTypes ++ [T])) :
+    {pmI with promotedTypes := pmI.promotedTypes ++ [T]}.refines
+      {pm with promotedTypes := pm.promotedTypes.tryPromote T} := by
+  have hbounds : pm.promotedTypes.strictly_bounds T := hrefines.strictly_bounds_iff.mp hchain
+  constructor <;> simp_all
+
+/--
+Conversely, in the circumstances in which the algorithm declines to promote a variable to `T` (that
+is, when appending `T` to its list of promoted types wouldn't produce a valid promotion chain),
+`PromotionChain.tryPromote` is a no-op.
+-/
+public theorem PromotionModelImpl.refines.tryPromote_eq_self {pmI : PromotionModelImpl}
+    {pm : PromotionModel} {T : τ} (hrefines : pmI.refines pm)
+    (hchain : ¬isPromotionChain (pmI.promotedTypes ++ [T])) :
+    pm.promotedTypes.tryPromote T = pm.promotedTypes := by
+  have hbounds : ¬pm.promotedTypes.strictly_bounds T := hrefines.strictly_bounds_iff.not.mp hchain
+  simp [hbounds]
+
+public theorem PromotionModelImpl.refines.join {pmI₁ pmI₂ : PromotionModelImpl}
+    {pm₁ pm₂ : PromotionModel} :
+    pmI₁.refines pm₁ → pmI₂.refines pm₂ → (pmI₁.join pmI₂).refines (pm₁.join pm₂) := by
+  rintro hrefines₁ hrefines₂
+  simp [PromotionModelImpl.join, PromotionModel.join]
+  constructor
+  case promotedTypes =>
+    simp [hrefines₁.promotedTypes, hrefines₂.promotedTypes]
+    rw [joinPromotedTypesImpl_pure_correct pm₁.promotedTypes pm₂.promotedTypes]
+  case tested =>
+    intro T; simp [joinTestedImpl, List.mem_union_iff, hrefines₁.tested, hrefines₂.tested]
+  case assigned => simp [hrefines₁.assigned, hrefines₂.assigned]
+  case unassigned => simp [hrefines₁.unassigned, hrefines₂.unassigned]
+  case version? => simp [hrefines₁.version?, hrefines₂.version?]
+
+end FlowAnalysis
